some suggestions in withScope.fst

examples/low-level/withScope.fst
@@ -1,5 +1,5 @@
 (*--build-config
-    options:--admit_fsi Set;
+    options:--admit_fsi Set --logQueries --debug Test --debug_level High --debug_level Rel;
     variables:LIB=../../lib;
     other-files:$LIB/ext.fst $LIB/set.fsi $LIB/heap.fst $LIB/st.fst $LIB/list.fst stack.fst listset.fst st3.fst
   --*)
@@ -14,21 +14,13 @@ open ListSet
 
 
 
-val withNewScope3 : a:Type ->
-   body:(unit -> SST a
-     (requires mStackNonEmpty)
-     (ensures (fun m0 _ m1 -> mStackNonEmpty m1))
-     )
+val withNewScope3 : #a:Type ->
+      body:(unit -> SST a mStackNonEmpty
+                          (fun m0 _ m1 -> mStackNonEmpty m1))
       -> SST a (requires (fun m -> True))
-                (ensures (fun m0 a m1 -> True))
+               (ensures (fun m0 a m1 -> True))
 
-let withNewScope3 (a:Type)
-  (body:(unit -> SST a
-          (requires mStackNonEmpty)
-          (ensures (fun _ _ m1 -> mStackNonEmpty m1)))
-          )
-          =
-(* omitting the types in above let expression results in a wierd error*)
+let withNewScope3 body =
     pushStackFrame ();
     let v = body () in
     popStackFrame (); v
@@ -40,67 +32,48 @@ let identity n = n
 
 
 val identity2  : n:nat -> unit ->
-   SST nat (fun m -> True /\ mStackNonEmpty m)
-              (fun _ n' m1 ->  n'=n /\ mStackNonEmpty m1)
+   SST nat (fun m -> mStackNonEmpty m)
+           (fun _ n' m1 ->  n'=n /\ mStackNonEmpty m1)
 let identity2 n u = n
 
 
 val scopedID : n:nat
-  -> SST nat (fun m -> True)
-              (fun _ n' _ -> n'==n)
-
+  -> SST nat (requires (fun m -> True))
+             (ensures (fun _ n' _ -> True)) // n'==n))
 (* This does not typecheck *)
-(*let scopedID (n:nat) =
-  withNewScope3
-    nat
-    (fun () ->  n)*)
-
-(* The part below also does not typecheck. The error is uninformative:
-Subtyping check failed; expected type (unit -> SST (nat)); got type (unit -> SST (nat))
-Perhaps some implicit argument is different
-
+(* NS: Why do you expect it to type-check? The post-condition of withNewScope3 is just True.
+       So, there's no way to prove that n=n' from that.
+       It does check if you remove that post-condition from scopedID *)
 let scopedID (n:nat) =
-  withNewScope3
-    nat
-     (identity2 n)*)
-
-
-
-let scopedID (n:nat) =
- withNewScope
-   nat
-   (fun m -> True)
-   (fun _ n' _ -> n'==n)
-   (fun () ->  n)
-
-
-(* Leaving the pre/post conditions out makes the above fail.
-   Having to put those everytime when callling withNewScope will be very tedious
-
-let scopedID (n:nat) =
- withNewScope
-   nat
-   _
-   _
-   (fun () ->  n)*)
-
-
-val scopedID2 : n:nat
-  -> SST nat (fun m -> True)
-              (fun _ n' _ -> True)
-
-let scopedID2 (n:nat) =
-  withNewScope3
-    nat
+  withNewScope3 #nat
     (fun () ->  n)
 
+(* NS: Here's how I would write it *)
+val withNewScope4 : #a:Type -> #req:(smem -> Type) -> #ens:(smem -> a -> smem -> Type)
+      -> =body:(unit -> SST a req ens) //=body is an equality constraint for type inference
+      -> SST a (requires (fun m ->
+                            (forall m'. mtail m' = m
+                                    /\ isNonEmpty (st m')
+                                    /\ topstb m' = emp
+                                    ==> req m')
+                         /\ (forall m0 x m1. ens m0 x m1 ==> sids m0 = sids m1)))
+               (ensures (fun m0 x m1 ->
+                         sids m0 = sids m1
+                         /\ (exists m0' m1'. mtail m0'=m0
+                                          /\ isNonEmpty (st m0')
+                                          /\ topstb m0'=emp
+                                          /\ ens m0' x m1')))
+let withNewScope4 body =
+   pushStackFrame ();
+   let v = body () in
+   popStackFrame (); v
 
-(*Just being able to define an abbreviation like below should be good, but it fails*)
-(*let withNewScope4
-  body
-          =
-    pushStackFrame ();
-    let v = body () in
-    popStackFrame (); v*)
-
-(*effect ALL and StSTATE cannot be combined*)
+val scopedID4 : n:nat
+ -> SST nat (requires (fun m -> True))
+            (ensures (fun _ n' _ -> n'==n))
+let scopedID4 (n:nat) =
+  //unfortunately, you still need to annotate the type of the argument to withNewScope4
+  //working on making inference compute it properly
+  let id : unit -> SST nat (fun s -> True) (fun s0 x s1 -> s0=s1 /\ x=n) =
+    fun () -> n in
+  withNewScope4 id
